C function restructured to be more succinct Uses a mix of if-then-else and match statements due to the abscence (in general or in documentation) of an otherwise statement in Dafny. Possibly not the final version.

config.dfy
@@ -46,27 +46,26 @@ type ClassId = int
 type VarId = int
 
 //type Class = map<ActorAddr, ClassId>
-/*
 //pass maps around?
-function sees(cl: Class, a: ActorAddr, sp: SP) : Capability
+//now that Class is not a map, sees needs the config 
+function sees(a: ActorAddr, sp: SP, c: Config) : Capability
 {
-    if a in cl then sees'(cl[a], sp) else Capability.ERR
+    //all_actors_in_config();
+    if 0 <= a < |c.actors| then sees'(c.actors[a].cl, sp) else Capability.ERR
 }
 
 function sees'(cid: ClassId, sp: SP) : Capability
 
-lemma A1(c: Config, cl: Class, a: ActorAddr, sp: SP, f: FId, cappa: Capability) 
-requires sees(cl, a, SP.cons(sp, f)) == cappa //pass cappa as param instead?
+lemma A1(c: Config, a: ActorAddr, sp: SP, f: FId, cappa: Capability) 
+requires sees(a, SP.cons(sp, f), c) == cappa //pass cappa as param instead?
 //requires sees(cl, c, a, SP.cons(sp, f)) == _ 
-ensures exists cappa' :: cappa' != TAG && sees(cl, a, sp) == cappa'
+ensures exists cappa' :: cappa' != TAG && sees(a, sp, c) == cappa'
 
-lemma A2(c: Config, cl: Class, a: ActorAddr, sp: SP, f: FId) 
-requires sees(cl, a, SP.cons(sp, f)) == WRITE
-ensures sees(cl, a, sp) == WRITE
+lemma A2(c: Config, a: ActorAddr, sp: SP, f: FId) 
+requires sees(a, SP.cons(sp, f), c) == WRITE
+ensures sees(a, sp, c) == WRITE
 
-
-/*
-function method C(a: ActorAddr, dp: DP, c: Config) : Addr 
+/*function method C_ver0(a: ActorAddr, dp: DP, c: Config) : Addr 
 {
     all_actors_in_config();
     match dp 
@@ -86,21 +85,46 @@ function method C(a: ActorAddr, dp: DP, c: Config) : Addr
         case trc(_) => Addr.ERR
         case mkR(_) => Addr.ERR
         case cll(_) => Addr.ERR
-}
+}*/
 
+
+//C FINAL 
+function method C(a: ActorAddr, dp: DP, c: Config) : Addr 
+{
+    all_actors_in_config();
+    match dp 
+    case This => AA(a)
+    case MP(k, x) => 
+        (MP_wf(c.actors[a], k);
+        var msg := c.actors[a].q[k];
+        if msg.app? then 
+            (if x in msg.f.Map then msg.f.Map[x] else Addr.ERR) 
+        else Addr.ERR)
+    case LP(zero, x) =>
+        (var state := c.actors[a].st;
+        if state.exe? then 
+            (if x in state.f.Map then state.f.Map[dp.x] else Addr.ERR)
+        else Addr.ERR)
+    case cons(p, f) => 
+        assume C(a, p, c) in c.heap.objs;
+        var obj := c.heap.objs[C(a, p, c)];
+        if f in obj then obj[f] else Addr.ERR
+}
 
 lemma MP_wf(a: Actor, k: int) 
 ensures 0 <= k < |a.q| 
 
 //can we assume this?
 lemma all_actors_in_config()
-ensures forall a: ActorAddr, c: Config :: a in c.actors
+ensures forall a: ActorAddr, c: Config :: 0 <= a < |c.actors|
 
 function method valid_addr(l: Addr) : bool {
     true
 }
 
-function method C(a: ActorAddr, dp: DP, c: Config) : Addr 
+/*
+//C: HELPER FUNCTIONS }
+function method C'(a: ActorAddr, dp: DP, c: Config) : Addr 
 {
     all_actors_in_config();
     match dp 
@@ -115,6 +139,7 @@ function method C(a: ActorAddr, dp: DP, c: Config) : Addr
         var obj := c.heap.objs[C(a, p, c)];
         if f in obj then obj[f] else Addr.ERR
 }
+
 function method CLP(zero: int, x: VarId, c: Config, a: Actor) : Addr
 {   
     match a.st 
@@ -136,4 +161,31 @@ requires 0 <= k < |a.q|
     case app(f) => if x in f.Map then f.Map[x] else Addr.ERR
     case orca(_, _) => Addr.ERR
 }
-*/
+
+
+//C: ALL IN ONE
+function method C''(a: ActorAddr, dp: DP, c: Config) : Addr 
+{
+    all_actors_in_config();
+    if dp.This? then 
+        AA(a) 
+    else if dp.MP? then (
+        MP_wf(c.actors[a], dp.k);
+        match c.actors[a].q[dp.k] 
+        case app(f) => if dp.x' in f.Map then f.Map[dp.x'] else Addr.ERR
+        case orca(_, _) => Addr.ERR
+        )
+    else if dp.LP? then (
+        match c.actors[a].st 
+        //add wf of frames?
+        case exe(f) => if dp.x in f.Map then f.Map[dp.x] else Addr.ERR
+        case snd(_, _, _, _) => Addr.ERR
+        case idl => Addr.ERR
+        case mkU(_) => Addr.ERR
+        case trc(_) => Addr.ERR
+        case mkR(_) => Addr.ERR
+        case cll(_) => Addr.ERR
+         )
+    else 
+       Addr.ERR
+}*/
